ImportTable

Auto/Embedding/LamChecker.lean
@@ -4,16 +4,18 @@ import Auto.Lib.BinTree
 namespace Auto.Embedding.Lam
 
 -- Table of valid propositions and well-formed formulas
--- Note that `Auto.BinTree α` is equivalent to `{n : Nat // n ≠ 0} → Option α`,
---   which means that
---   1. Index `0` is not present. Inserting element to index `0` does nothing,
---      and retrieving element from index `0` produces `.none`
---   2. `.some` entries may be interspersed with `.none` entries
+-- Note that `Auto.BinList α` is equivalent to `Nat → Option α`,
+--   which means that `.some` entries may be interspersed
+--   with `.none` entries
 structure RTable where
   -- Well-formed formulas, with types
-  wf    : Auto.BinTree (List LamSort × LamSort × LamTerm)
+  -- We do not import well-formedness facts because
+  --   we have `LamWF.ofCheck?`
+  wf    : Auto.BinList (List LamSort × LamSort × LamTerm)
   -- Valid propositions
-  valid : Auto.BinTree (List LamSort × LamTerm)
+  -- The initial formulas in the `valid` table will be
+  --   imported from `ImportTable`
+  valid : Auto.BinList (List LamSort × LamTerm)
 
 -- An entry of RTable
 inductive REntry where
@@ -29,18 +31,46 @@ def RTable.addEntry (r : RTable) (n : Nat) : REntry → RTable
 -- Invariant of `wf`
 def RTable.wfInv
   (lval : LamValuation.{u})
-  (wf : Auto.BinTree (List LamSort × LamSort × LamTerm)) :=
+  (wf : Auto.BinList (List LamSort × LamSort × LamTerm)) :=
   wf.allp (fun ⟨lctx, rty, t⟩ => LamThmWF' lval lctx rty t)
 
 -- Invariant of `valid
 def RTable.validInv
   (lval : LamValuation.{u})
-  (valid : Auto.BinTree (List LamSort × LamTerm)) :=
+  (valid : Auto.BinList (List LamSort × LamTerm)) :=
   valid.allp (fun ⟨lctx, t⟩ => LamThmValid lval lctx t)
 
 -- Invariant of `RTable`
 def RTable.inv (lval : LamValuation.{u}) (r : RTable) :=
   wfInv lval r.wf ∧ validInv lval r.valid
+
+-- The meta code of the checker will prepare this `ImportTable`
+abbrev ImportTable (lval : LamValuation.{u}) :=
+  Auto.BinList (@PSigma LamTerm (fun p => (LamTerm.interpAsProp lval dfLCtxTy (dfLCtxTerm _) p).down))
+
+def RTable.importFacts (it : ImportTable lval) : BinList (List LamSort × LamTerm) :=
+  it.mapOpt (fun ⟨p, _⟩ =>
+    match p.lamCheck? lval.ilVal.toLamTyVal dfLCtxTy with
+    | .some (.base .prop) =>
+      match p.maxLooseBVarSucc with
+      | 0 => .some ([], p)
+      | _ + 1 => .none
+    | _                   => .none)
+
+theorem RTable.import_correct (it : ImportTable lval) :
+  RTable.validInv lval (importFacts it) := by
+  dsimp [RTable.validInv, importFacts]; rw [BinList.mapOpt_allp]
+  intro n; apply Option.allp_uniform;
+  intro ⟨p, validp⟩; dsimp
+  cases h₁ : LamTerm.lamCheck? lval.ilVal.toLamTyVal dfLCtxTy p <;> try exact True.intro
+  case a.some s =>
+    cases s <;> try exact True.intro
+    case base b =>
+      cases b <;> try exact True.intro
+      dsimp
+      cases h₂ : p.maxLooseBVarSucc <;> try exact True.intro
+      dsimp [Option.allp]
+      apply LamThmValid.ofInterpAsProp _ _ h₁ validp h₂    
 
 inductive ChkStep where
   -- Adds `⟨lctx, t, t.lamCheck!⟩` to `rtable.wf`
