Auto/Lib/OptionExtra.lean
@@ -4,12 +4,18 @@ namespace Auto
   | some a => p a
   | none   => True
 
-theorem Option.p_all_eq_true (p : α → Bool) (x : Option α) :
+theorem Option.all_allp (p : α → Bool) (x : Option α) :
   (x.all p = true) = Option.allp (fun x => p x = true) x :=
   match x with
   | .none => by
     dsimp [Option.all, Option.allp]; simp
   | .some x => by
     dsimp [Option.all, Option.allp]
+
+theorem Option.allp_uniform (p : α → Prop) (x : Option α) :
+  (∀ (x : α), p x) → Option.allp p x := by
+  cases x <;> intro h
+  case none => exact True.intro
+  case some v => apply h
 
 end Auto
